test function that receives two flights

src/tls/experiments/HSL.Receive.Wrapper.fst
@@ -31,24 +31,41 @@ noeq type rcv_state = {
 /// In case of partially parsed flights, the prefix [rcv_from, Rcv.length_parsed_bytes]
 ///   is what HSL.Receive maintains
 
-let rcv_inv (st:rcv_state) (h:HS.mem) : Type0 =
+let rcv_reset_inv (st:rcv_state) (h:HS.mem) : Type0 =
+  B.live h st.rcv_b /\
+  Rcv.invariant st.hsl_rcv_st h /\
+  Rcv.parsed_bytes st.hsl_rcv_st h == Seq.empty /\
+  Rcv.in_progress_flt st.hsl_rcv_st h == Rcv.F_none
+
+let rcv_in_progress_inv (st:rcv_state) (h:HS.mem) : Type0 =
   B.live h st.rcv_b /\
   Rcv.invariant st.hsl_rcv_st h /\
   Rcv.length_parsed_bytes st.hsl_rcv_st h <= (v st.rcv_to - v st.rcv_from) /\
   Rcv.parsed_bytes st.hsl_rcv_st h ==
     Seq.slice (B.as_seq h st.rcv_b) (v st.rcv_from) (v st.rcv_from + Rcv.length_parsed_bytes st.hsl_rcv_st h) /\
-  ((Rcv.in_progress_flt st.hsl_rcv_st h == Rcv.F_none) \/
-   (Rcv.in_progress_flt st.hsl_rcv_st h == G.reveal st.current_flt))
+  Rcv.in_progress_flt st.hsl_rcv_st h == G.reveal st.current_flt
 
+let invariant (st:rcv_state) (h:HS.mem) =
+  rcv_reset_inv st h \/ rcv_in_progress_inv st h
 
-let frame_rcv_inv
+let frame_rcv_reset_inv
   (st:rcv_state) (l:B.loc) (h0 h1:HS.mem)
   : Lemma
     (requires
-      rcv_inv st h0 /\
+      rcv_reset_inv st h0 /\
       B.(loc_disjoint (loc_union (Rcv.footprint st.hsl_rcv_st) (loc_buffer st.rcv_b)) l /\
       B.modifies l h0 h1))
-    (ensures rcv_inv st h1 /\ B.as_seq h0 st.rcv_b == B.as_seq h1 st.rcv_b)
+    (ensures rcv_reset_inv st h1 /\ B.as_seq h0 st.rcv_b == B.as_seq h1 st.rcv_b)
+  = Rcv.frame_hsl_state st.hsl_rcv_st h0 h1 l
+
+let frame_rcv_in_progress_inv
+  (st:rcv_state) (l:B.loc) (h0 h1:HS.mem)
+  : Lemma
+    (requires
+      rcv_in_progress_inv st h0 /\
+      B.(loc_disjoint (loc_union (Rcv.footprint st.hsl_rcv_st) (loc_buffer st.rcv_b)) l /\
+      B.modifies l h0 h1))
+    (ensures rcv_in_progress_inv st h1 /\ B.as_seq h0 st.rcv_b == B.as_seq h1 st.rcv_b)
   = Rcv.frame_hsl_state st.hsl_rcv_st h0 h1 l
 
 let create
@@ -62,7 +79,7 @@ let create
       Rcv.parsed_bytes hsl_rcv_st h == Seq.empty)
     (ensures fun h0 st h1 ->
       h0 == h1 /\
-      rcv_inv st h1 /\
+      rcv_reset_inv st h1 /\
       st == {
         current_flt = G.hide Rcv.F_none;
         hsl_rcv_st = hsl_rcv_st;
@@ -83,7 +100,6 @@ unfold let only_increments_rcv_to (st1 st0:rcv_state) =
   st1.rcv_from == st0.rcv_from /\
   st0.rcv_to <= st1.rcv_to
 
-
 private let lemma_seq (#a:Type) (s1 s2:Seq.seq a) (from to:nat) (to':nat)
   : Lemma
     (requires
@@ -98,44 +114,116 @@ let buffer_received_fragment
   (st:rcv_state) (bs:bytes)
   : Stack rcv_state
     (requires fun h ->
-      rcv_inv st h /\
-      Bytes.length bs <> 0 /\  //required by FStar.Bytes.store_bytes
+      invariant st h /\
       v st.rcv_to + Bytes.length bs <= B.length st.rcv_b)  //that adding these bytes does not overflow the buffer
     (ensures fun h0 rst h1 ->
-      rcv_inv rst h1 /\
-      rst `only_increments_rcv_to` st /\
-      B.(modifies (loc_buffer (gsub st.rcv_b st.rcv_to (Bytes.len bs)))) h0 h1 /\
-      Seq.slice (B.as_seq h1 rst.rcv_b) (v st.rcv_to) (v rst.rcv_to) == Bytes.reveal bs)
-  = let h0 = ST.get () in
+      if Bytes.length bs = 0 then h0 == h1 /\ rst == st
+      else
+        rst `only_increments_rcv_to` st /\
+        rst.rcv_to == st.rcv_to + Bytes.len bs /\
+        B.(modifies (loc_buffer (gsub st.rcv_b st.rcv_to (Bytes.len bs)))) h0 h1 /\
+        Seq.slice (B.as_seq h1 rst.rcv_b) (v st.rcv_to) (v rst.rcv_to) == Bytes.reveal bs /\
+        invariant rst h1)
+  = if Bytes.length bs = 0 then st
+    else
+      let h0 = ST.get () in
+      let sub = B.sub st.rcv_b st.rcv_to (Bytes.len bs) in
+      FStar.Bytes.store_bytes bs sub;
+      let h1 = ST.get () in
+      Rcv.frame_hsl_state st.hsl_rcv_st h0 h1 (B.loc_buffer sub);
+      let rst = { st with rcv_to = st.rcv_to + Bytes.len bs } in
 
-    let sub = B.sub st.rcv_b st.rcv_to (Bytes.len bs) in
-    FStar.Bytes.store_bytes bs sub;
+      assert (Seq.equal (B.as_seq h1 (B.gsub rst.rcv_b rst.rcv_from (st.rcv_to - rst.rcv_from)))
+                       (Seq.slice (B.as_seq h1 rst.rcv_b) (v rst.rcv_from) (v st.rcv_to)));
+      lemma_seq
+        (B.as_seq h0 st.rcv_b)
+        (B.as_seq h1 rst.rcv_b)
+        (v st.rcv_from)
+        (v st.rcv_to)
+        (v st.rcv_from + Rcv.length_parsed_bytes st.hsl_rcv_st h0);
+      rst
 
-    let h1 = ST.get () in
- 
-    Rcv.frame_hsl_state st.hsl_rcv_st h0 h1 (B.loc_buffer sub);
-    
-    let rst = { st with rcv_to = st.rcv_to + Bytes.len bs } in
 
-    assert (Seq.equal (B.as_seq h1 (B.gsub rst.rcv_b rst.rcv_from (st.rcv_to - rst.rcv_from)))
-                      (Seq.slice (B.as_seq h1 rst.rcv_b) (v rst.rcv_from) (v st.rcv_to)));
-    lemma_seq
-      (B.as_seq h0 st.rcv_b)
-      (B.as_seq h1 rst.rcv_b)
-      (v st.rcv_from) 
-      (v st.rcv_to)
-      (v st.rcv_from + Rcv.length_parsed_bytes st.hsl_rcv_st h0);
+module HSM = Parsers.Handshake
+module R = MITLS.Repr
+module C = LowStar.ConstBuffer
 
-    rst
 
-// module HSM = Parsers.Handshake
+let cslice_of (st:rcv_state) : R.const_slice =
+  assume (st.rcv_to <= LP.validator_max_length);
+  R.MkSlice (C.of_buffer st.rcv_b) st.rcv_to
 
-// type sh_flight = {
-//   sh : m:HSM.handshake{HSM.M_server_hello? m}
-// }
+let receive_c_wait_ServerHello
+  (st:rcv_state)
+  : ST (TLSError.result (option ((Rcv.c_wait_ServerHello (cslice_of st)) & uint_32)))
+    (requires fun h ->
+      G.reveal st.current_flt == Rcv.F_c_wait_ServerHello /\
+      (rcv_reset_inv st h \/ rcv_in_progress_inv st h))
+    (ensures fun h0 r h1 ->
+      B.modifies (Rcv.footprint st.hsl_rcv_st) h0 h1 /\
+      (let open FStar.Error in
+       match r with
+       | Error _ -> True
+       | Correct None ->
+         rcv_in_progress_inv st h1
+       | Correct (Some (flt, idx_end)) ->
+         idx_end <= st.rcv_to /\
+         Rcv.valid_c_wait_ServerHello st.rcv_from idx_end flt h1 /\
+         rcv_reset_inv st h1))
+  = Rcv.receive_c_wait_ServerHello st.hsl_rcv_st (cslice_of st) st.rcv_from st.rcv_to
 
-// let receive_c_wait_ServerHello
-//   (st:rcv_state)
-//   : ST (TLSError.result (option (sh_flight & uint_32)))
-//     (requires fun h ->
-//       rcv_inv st h /\
+let receive_c12_wait_ServerHelloDone
+  (st:rcv_state)
+  : ST (TLSError.result (option (Rcv.c12_wait_ServerHelloDone (cslice_of st))))
+    (requires fun h ->
+      G.reveal st.current_flt == Rcv.F_c12_wait_ServerHelloDone /\
+      (rcv_reset_inv st h \/ rcv_in_progress_inv st h))
+    (ensures fun h0 r h1 ->
+      B.modifies (Rcv.footprint st.hsl_rcv_st) h0 h1 /\
+      (let open FStar.Error in
+       match r with
+       | Error _ -> True
+       | Correct None ->
+         rcv_in_progress_inv st h1
+       | Correct (Some flt) ->
+         Rcv.valid_c12_wait_ServerHelloDone st.rcv_from st.rcv_to flt h1 /\
+         rcv_reset_inv st h1))
+  = Rcv.receive_c12_wait_ServerHelloDone st.hsl_rcv_st (cslice_of st) st.rcv_from st.rcv_to
+
+assume val bs : bytes
+
+let test_change_of_flight (st:rcv_state) : St unit =
+  let open FStar.Error in
+  (*
+   * assume that the state is in the reset state, i.e. no flight in progress
+   * this is what you get when rcv_state is created
+   *)
+  let h = ST.get () in
+  assume (rcv_reset_inv st h);
+
+  (* try to receive ServerHello *)
+  let st = { st with current_flt = G.hide Rcv.F_c_wait_ServerHello } in
+  let r = receive_c_wait_ServerHello st in
+  match r with
+  | Error e -> ()  //abandon
+  | Correct None ->
+    //waiting for more data
+    //append some bytes
+    assume (v st.rcv_to + Bytes.length bs <= B.length st.rcv_b);
+    let st = buffer_received_fragment st bs in
+    //call receive again
+    let r = receive_c_wait_ServerHello st in
+    ()  //and so on
+  | Correct (Some (flt, idx_end)) ->
+    //flt is a valid ServerHello flight
+    //now let's try to parse ServerHelloDone
+    let st = { st with
+      current_flt = G.hide Rcv.F_c12_wait_ServerHelloDone;
+      rcv_from = idx_end } in
+
+    let r = receive_c12_wait_ServerHelloDone st in
+    ()  //and so on
+
+
+
+
